theories/typing/array.v
@@ -1,16 +1,102 @@
 From lrust.typing Require Export type.
-From lrust.typing Require Import product mod_ty.
+From lrust.typing Require Import product.
 Set Default Proof Using "Type".
+
+Implicit Type 𝔄 𝔅 ℭ: syn_type.
 
 Section array.
   Context `{!typeG Σ}.
 
-  Definition array {𝔄} n (ty: type 𝔄) : type (Π! (trepeat 𝔄 n)) := Π! (hrepeat ty n).
+  Lemma split_array_mt {𝔄 n} (ty: type 𝔄) l q (aπl: _ n) d tid :
+    (l ↦∗{q}: λ vl, ∃wll: vec _ _, ⌜vl = concat wll⌝ ∗
+      [∗ list] aπwl ∈ vzip aπl wll, ty.(ty_own) aπwl.1 d tid aπwl.2)%I ⊣⊢
+    [∗ list] i ↦ aπ ∈ aπl,
+      (l +ₗ (i * ty.(ty_size))%nat) ↦∗{q}: ty.(ty_own) aπ d tid.
+  Proof. iSplit.
+    - iIntros "(%& ↦s &%&->& tys)". iInduction aπl as [] "IH" forall (l);
+      inv_vec wll; [done|]=>/= ??. iRevert "↦s tys".
+      rewrite heap_mapsto_vec_app. iIntros "[↦ ↦s][ty tys]".
+      iDestruct (ty_size_eq with "ty") as %->. iSplitL "↦ ty".
+      { iExists _. rewrite shift_loc_0. iFrame. }
+      setoid_rewrite <-shift_loc_assoc_nat. iApply ("IH" with "↦s tys").
+    - iIntros "↦owns". iInduction aπl as [] "IH" forall (l)=>/=.
+      { iExists []. iSplitR; by [rewrite heap_mapsto_vec_nil|iExists [#]=>/=]. }
+      iDestruct "↦owns" as "[(%& ↦ & ty) ↦owns]".
+      rewrite shift_loc_0. setoid_rewrite <-shift_loc_assoc_nat.
+      iDestruct ("IH" with "↦owns") as (?) "(↦s &%&->& tys)". iExists (_++_).
+      rewrite heap_mapsto_vec_app. iDestruct (ty_size_eq with "ty") as %->.
+      iFrame "↦ ↦s". iExists (_:::_). iSplit; [done|]. iFrame.
+  Qed.
+
+  Definition vfunsep' {𝔄 n} : proph (vecₛ 𝔄 n) → vec (proph 𝔄) n := vfunsep.
+
+  Program Definition array {𝔄} n (ty: type 𝔄) : type (vecₛ 𝔄 n) := {|
+    ty_size := n * ty.(ty_size);  ty_lfts := ty.(ty_lfts);  ty_E := ty.(ty_E);
+    ty_own vπ d tid vl := ∃wll: vec _ _, ⌜vl = concat wll⌝ ∗
+      [∗ list] aπwl ∈ vzip (vfunsep' vπ) wll, ty.(ty_own) aπwl.1 d tid aπwl.2;
+    ty_shr vπ d κ tid l := [∗ list] i ↦ aπ ∈ vfunsep' vπ,
+      ty.(ty_shr) aπ d κ tid (l +ₗ (i * ty.(ty_size))%nat);
+  |}%I.
+  Next Obligation.
+    iIntros "* (%&->& All)". setoid_rewrite ty_size_eq. move: {vπ}(vfunsep' vπ)=> aπl.
+    iInduction aπl as [] "IH"; inv_vec wll; [done|]=>/= ??. rewrite/= app_length.
+    iDestruct "All" as "[-> All]". by iDestruct ("IH" with "All") as %->.
+  Qed.
+  Next Obligation. move=>/= *. do 6 f_equiv. by apply ty_own_depth_mono. Qed.
+  Next Obligation. move=>/= *. do 3 f_equiv. by apply ty_shr_depth_mono. Qed.
+  Next Obligation.
+    iIntros "* #In". rewrite !big_sepL_forall. iIntros "All %%%".
+    iApply (ty_shr_lft_mono with "In"). by iApply "All".
+  Qed.
+  Next Obligation.
+    iIntros (??????? l ? q ?) "#LFT #In Bor κ". rewrite split_array_mt.
+    iMod (bor_big_sepL with "LFT Bor") as "Bors"; [done|].
+    move: {vπ}(vfunsep' vπ)=> aπl. iInduction aπl as [|] "IH" forall (l q)=>/=.
+    { iApply step_fupdN_full_intro. by iFrame. }
+    iDestruct "κ" as "[κ κ+]". iDestruct "Bors" as "[Bor Bors]".
+    iMod (ty_share with "LFT In Bor κ") as "Toshr"; [done|].
+    setoid_rewrite <-shift_loc_assoc_nat. iMod ("IH" with "κ+ Bors") as "Toshrs".
+    iCombine "Toshr Toshrs" as "Toshrs". iApply (step_fupdN_wand with "Toshrs").
+    by iIntros "!> [>[$$] >[$$]]".
+  Qed.
+  Next Obligation.
+    iIntros (????????? q ?) "#LFT #In (%&->& tys) κ".
+    have <-: vapply (vfunsep' vπ) = vπ by rewrite semi_iso'.
+    move: {vπ}(vfunsep' vπ)=> aπl. iInduction aπl as [] "IH" forall (q); inv_vec wll=>/=.
+    { iApply step_fupdN_full_intro. iIntros "!>!>". iExists [], 1%Qp.
+      do 2 (iSplitR; [done|]). iIntros "_!>". iFrame "κ". by iExists [#]=>/=. }
+    move=> ??. iDestruct "κ" as "[κ κ+]". iDestruct "tys" as "[ty tys]".
+    iMod (ty_own_proph with "LFT In ty κ") as "Toty"; [done|].
+    iMod ("IH" with "tys κ+") as "Totys". iCombine "Toty Totys" as "Totys".
+    iApply (step_fupdN_wand with "Totys").
+    iIntros "!>[>(%&%&%& ξl & Toty) >(%&%&%& ζl & Totys)] !>".
+    iDestruct (proph_tok_combine with "ξl ζl") as (?) "[ξζl Toξζl]".
+    iExists _, _. iSplit. { iPureIntro. by apply proph_dep_vcons. }
+    iFrame "ξζl". iIntros "ξζl". iDestruct ("Toξζl" with "ξζl") as "[ξl ζl]".
+    iMod ("Toty" with "ξl") as "[ty $]".
+    iMod ("Totys" with "ζl") as "[(%wll &%& tys) $]". iModIntro.
+    iExists (_ ::: wll). iSplitR; [iPureIntro=>/=; by f_equal|]. iFrame.
+  Qed.
+  Next Obligation.
+    iIntros (???????? l ? q ?) "#LFT #In #In' tys κ'".
+    have <-: vapply (vfunsep' vπ) = vπ by rewrite semi_iso'.
+    move: {vπ}(vfunsep' vπ)=> aπl. iInduction aπl as [] "IH" forall (q l)=>/=.
+    { iApply step_fupdN_full_intro. iIntros "!>!>!>!>". iExists [], 1%Qp.
+      do 2 (iSplitR; [done|]). iIntros "_!>". iFrame. }
+    iDestruct "κ'" as "[κ' κ'+]". iDestruct "tys" as "[ty tys]".
+    iMod (ty_shr_proph with "LFT In In' ty κ'") as "Toty"; [done|].
+    setoid_rewrite <-shift_loc_assoc_nat. iMod ("IH" with "tys κ'+") as "Totys".
+    iCombine "Toty Totys" as "Totys". iIntros "!>!>".
+    iApply (step_fupdN_wand with "Totys").
+    iIntros "[>(%&%&%& ξl & Toty) >(%&%&%& ζl & Totys)] !>".
+    iDestruct (proph_tok_combine with "ξl ζl") as (?) "[ξζl Toξζl]".
+    iExists _, _. iSplit. { iPureIntro. by apply proph_dep_vcons. }
+    iFrame "ξζl". iIntros "ξζl". iDestruct ("Toξζl" with "ξζl") as "[ξl ζl]".
+    iMod ("Toty" with "ξl") as "[$$]". by iMod ("Totys" with "ζl") as "[$$]".
+  Qed.
 
   Global Instance array_ne {𝔄} n : NonExpansive (@array 𝔄 n).
-  Proof.
-    elim n; [by constructor|]=> ? Eq' ??? Eq. apply (.$ Eq) in Eq'. solve_ne_type.
-  Qed.
+  Proof. solve_ne_type. Qed.
 
 End array.
 
@@ -20,32 +106,81 @@ Section typing.
   Context `{!typeG Σ}.
 
   Global Instance array_type_ne {𝔄} n : TypeNonExpansive (@array _ _ 𝔄 n).
-  Proof. elim n; apply _. Qed.
+  Proof.
+    split; [by apply type_lft_morph_id_like|by move=>/= ??->| | ]=>/= > Sz *;
+    [by do 6 f_equiv|rewrite Sz; by do 3 f_equiv].
+  Qed.
+
   Global Instance array_copy {𝔄} n (ty: _ 𝔄) : Copy ty → Copy [ty; n].
-  Proof. elim n; apply _. Qed.
+  Proof.
+    split; [apply _|]=>/= vπ ???? F l q ? HF. iIntros "#LFT tys Na κ".
+    move: {vπ}(vfunsep' vπ)=> aπl. iInduction aπl as [] "IH" forall (q l F HF)=>/=.
+    { iModIntro. iExists 1%Qp, []. rewrite difference_empty_L heap_mapsto_vec_nil.
+      iFrame "Na κ". iSplitR; [by iExists [#]=>/=|]. by iIntros. }
+    rewrite shift_loc_0. iDestruct "tys" as "[ty tys]". iDestruct "κ" as "[κ κ+]".
+    iMod (copy_shr_acc with "LFT ty Na κ") as (q' ?) "(Na & ↦ & #ty & Toκ)";
+    [done| |]. { rewrite <-HF. apply shr_locsE_subseteq=>/=. lia. }
+    setoid_rewrite <-shift_loc_assoc_nat.
+    iMod ("IH" with "[%] tys Na κ+") as (q'' ?) "(Na & ↦' & (%&>->& #tys) & Toκ+)".
+    { apply subseteq_difference_r. { symmetry. apply shr_locsE_disj. }
+      move: HF. rewrite -plus_assoc shr_locsE_shift. set_solver. }
+    case (Qp_lower_bound q' q'')=> [q'''[?[?[->->]]]]. iExists q''', (_ ++ _).
+    rewrite heap_mapsto_vec_app. iDestruct (ty_size_eq with "ty") as ">->".
+    iDestruct "↦" as "[$ ↦r]". iDestruct "↦'" as "[$ ↦r']".
+    iDestruct (na_own_acc with "Na") as "[$ ToNa]".
+    { rewrite shr_locsE_shift. set_solver. } iSplitR.
+    { iIntros "!>!>". iExists (_:::_)=>/=. iSplit; by [|iSplit]. }
+    iIntros "!> Na [↦ ↦']". iDestruct ("ToNa" with "Na") as "Na".
+    iMod ("Toκ+" with "Na [$↦' $↦r']") as "[Na $]". iApply ("Toκ" with "Na [$↦ $↦r]").
+  Qed.
+
   Global Instance array_send {𝔄} n (ty: _ 𝔄) : Send ty → Send [ty; n].
-  Proof. elim n; apply _. Qed.
+  Proof. move=> >/=. by do 6 f_equiv. Qed.
   Global Instance array_sync {𝔄} n (ty: _ 𝔄) : Sync ty → Sync [ty; n].
-  Proof. elim n; apply _. Qed.
+  Proof. move=> >/=. by do 3 f_equiv. Qed.
 
   Lemma array_subtype {𝔄 𝔅} E L n (f: 𝔄 → 𝔅) ty ty' :
-    subtype E L f ty ty' → subtype E L (f -v<$>.) [ty; n] [ty'; n].
-  Proof. move=> ?. elim: n; [done|]=>/= ??. by apply cons_prod_subtype. Qed.
+    subtype E L ty ty' f → subtype E L [ty; n] [ty'; n] (vmap f).
+  Proof.
+    iIntros (Sub ?) "L". iDestruct (Sub with "L") as "#Sub".
+    iIntros "!> E". iDestruct ("Sub" with "E") as "(%Sz & ? & #InOwn & #InShr)".
+    iSplit; [by rewrite/= Sz|]. iSplit; [done|].
+    have Eq: ∀vπ, vfunsep' (vmap f ∘ vπ) = vmap (f ∘.) (vfunsep' vπ).
+    { move=> ? vπ. have {1}<-: vapply (vfunsep' vπ) = vπ by rewrite semi_iso'.
+      move: (vfunsep' vπ)=> aπl. by elim aπl; [done|]=>/= ???<-. }
+    iSplit; iIntros "!> %vπ %/="; rewrite Eq; move: {vπ}(vfunsep' vπ)=> aπl.
+    - iIntros "* (%wll &->& tys)". iExists _. iSplit; [done|].
+      iInduction aπl as [] "IH"; inv_vec wll; [done|]=>/= ??.
+      iDestruct "tys" as "[ty tys]". iSplitL "ty"; by [iApply "InOwn"|iApply "IH"].
+    - iIntros "%% %l". iInduction aπl as [] "IH" forall (l); [by iIntros|]=>/=.
+      iIntros "[#ty #tys]". rewrite Sz. setoid_rewrite <-shift_loc_assoc_nat.
+      iSplitL "ty"; by [iApply "InShr"|iApply "IH"].
+  Qed.
   Lemma array_eqtype {𝔄 𝔅} E L n (f: 𝔄 → 𝔅) g ty ty' :
-    eqtype E L f g ty ty' → eqtype E L (f -v<$>.) (g -v<$>.) [ty; n] [ty'; n].
+    eqtype E L ty ty' f g → eqtype E L [ty; n] [ty'; n] (vmap f) (vmap g).
   Proof. move=> [??]. split; by apply array_subtype. Qed.
 
   Lemma array_plus_prod {𝔄} E L m n (ty: _ 𝔄) :
-    eqtype E L pvsep (curry pvapp) [ty; m + n] ([ty; m] * [ty; n]).
-  Proof. elim: m=> [|? Eq].
-    - eapply eqtype_eq. { eapply eqtype_trans;
-      [apply eqtype_symm; apply prod_ty_left_id|]. apply prod_eqtype; [|done].
-      apply mod_ty_inout, _. } { done. } { done. }
-    - eapply eqtype_eq. { eapply eqtype_trans; [by apply mod_ty_outin, _|].
-      eapply eqtype_trans. { eapply prod_eqtype; [reflexivity|apply Eq]. }
-      eapply eqtype_trans; [by apply prod_ty_assoc|]. apply prod_eqtype;
-      [apply mod_ty_inout, _|done]. } { fun_ext. by case. }
-      { fun_ext. by case=> [[??]?]. }
+    eqtype E L [ty; m + n] ([ty; m] * [ty; n]) (vsepat m) (curry vapp).
+  Proof.
+    apply eqtype_symm, eqtype_unfold; [apply _|]. iIntros (?) "_!>_".
+    iSplit; [iPureIntro=>/=; lia|]. iSplit. { rewrite/= lft_intersect_list_app.
+    iApply lft_intersect_equiv_idemp. }
+    have Eq: ∀vπ: proph (vec 𝔄 _ * _), vfunsep' (curry vapp ∘ vπ) =
+      vfunsep' (fst ∘ vπ) +++ vfunsep' (snd ∘ vπ).
+    { move=> ?? vπ. have {1}<-: pair ∘ vapply (vfunsep' $ fst ∘ vπ) ⊛
+      vapply (vfunsep' $ snd ∘ vπ) = vπ by rewrite !semi_iso' -surjective_pairing_fun.
+      move: (_ $ fst ∘ _)=> aπl. by elim aπl; [by rewrite semi_iso'|]=>/= ???<-. }
+    iSplit; iIntros "!> %vπ %/="; rewrite Eq; move: (vfunsep' (fst ∘ vπ))=> aπl;
+    move: {vπ}(vfunsep' (snd ∘ vπ))=> bπl; iIntros "*"; [iSplit|].
+    - iIntros "(%&%&->&(%&->&?)&(%&->&?))". iExists (_+++_).
+      rewrite vzip_with_app !vec_to_list_app concat_app. by iFrame.
+    - iIntros "(%wll &->& tys)". move: (vapp_ex wll)=> [?[?->]].
+      rewrite vzip_with_app !vec_to_list_app concat_app. iExists _, _. iSplit; [done|].
+      iDestruct "tys" as "[tys tys']". iSplitL "tys"; iExists _; by iFrame.
+    - rewrite vec_to_list_app big_sepL_app vec_to_list_length.
+      setoid_rewrite shift_loc_assoc_nat. setoid_rewrite Nat.mul_add_distr_r.
+      by iApply (bi.iff_refl True%I).
   Qed.
 
 End typing.
